Software Foundations/lf/Maps.v
@@ -187,7 +187,10 @@ Proof. reflexivity. Qed.
 Lemma t_apply_empty : forall (A : Type) (x : string) (v : A),
   (__ !-> v) x = v.
 Proof.
-  (* FILL IN HERE *) Admitted.
+  intros.
+  reflexivity.
+Qed.
+
 (** [] *)
 
 (** **** Exercise: 2 stars, standard, optional (t_update_eq)
@@ -199,7 +202,12 @@ Proof.
 Lemma t_update_eq : forall (A : Type) (m : total_map A) x v,
   (x !-> v ; m) x = v.
 Proof.
-  (* FILL IN HERE *) Admitted.
+  intros.
+  unfold t_update.
+  rewrite (String.eqb_refl).
+  reflexivity.
+Qed.
+
 (** [] *)
 
 (** **** Exercise: 2 stars, standard, optional (t_update_neq)
@@ -212,7 +220,13 @@ Theorem t_update_neq : forall (A : Type) (m : total_map A) x1 x2 v,
   x1 <> x2 ->
   (x1 !-> v ; m) x2 = m x2.
 Proof.
-  (* FILL IN HERE *) Admitted.
+  intros.
+  unfold t_update.
+  apply String.eqb_neq in H.
+  rewrite H.
+  reflexivity.
+Qed.
+
 (** [] *)
 
 (** **** Exercise: 2 stars, standard, optional (t_update_shadow)
@@ -243,7 +257,19 @@ Proof.
 Theorem t_update_same : forall (A : Type) (m : total_map A) x,
   (x !-> m x ; m) = m.
 Proof.
-  (* FILL IN HERE *) Admitted.
+  intros.
+  assert (P : forall y, (x !-> m x ; m) y = m y). {
+    intros.
+    destruct (eqb_spec x y) as [Hxy | Hxy].
+    - rewrite Hxy. rewrite t_update_eq. reflexivity.
+    - rewrite t_update_neq.
+      + reflexivity.
+      + apply Hxy.
+  }
+  apply functional_extensionality. intros y.
+  apply P.
+Qed.
+
 (** [] *)
 
 (** **** Exercise: 3 stars, standard, especially useful (t_update_permute)
@@ -259,7 +285,25 @@ Theorem t_update_permute : forall (A : Type) (m : total_map A)
   =
   (x2 !-> v2 ; x1 !-> v1 ; m).
 Proof.
-  (* FILL IN HERE *) Admitted.
+  intros.
+  apply functional_extensionality.
+  intros.
+  destruct (eqb_spec x1 x) as [E | N].
+  - rewrite E. unfold t_update.
+    rewrite (eqb_refl x).
+    assert (Nb : (x2 =? x)%string = false). {
+      apply eqb_neq. rewrite <- E. apply H.
+    }
+    rewrite Nb.
+    reflexivity.
+  - unfold t_update.
+    assert (Nb : (x1 =? x)%string = false). {
+      apply eqb_neq. apply N.
+    }
+    rewrite Nb.
+    reflexivity.
+Qed.
+
 (** [] *)
 
 (* ################################################################# *)
