Software Foundations/lf/Rel.v
@@ -105,13 +105,16 @@ Proof.
 (** Copy the definition of [total_relation] from your [IndProp]
     here so that this file can be graded on its own.  *)
 Inductive total_relation : nat -> nat -> Prop :=
-  (* FILL IN HERE *)
-.
+  | just m n : total_relation m n.
 
 Theorem total_relation_not_partial_function :
   ~ (partial_function total_relation).
 Proof.
-  (* FILL IN HERE *) Admitted.
+  unfold not.
+  intros.
+  discriminate ((H 0 1 2) (just 0 1) (just 0 2)).
+Qed.
+
 (** [] *)
 
 (** **** Exercise: 2 stars, standard, optional (empty_relation_partial_function)
@@ -121,14 +124,16 @@ Proof.
 
 (** Copy the definition of [empty_relation] from your [IndProp]
     here so that this file can be graded on its own.  *)
-Inductive empty_relation : nat -> nat -> Prop :=
-  (* FILL IN HERE *)
-.
+Inductive empty_relation : nat -> nat -> Prop :=.
 
 Theorem empty_relation_partial_function :
   partial_function empty_relation.
 Proof.
-  (* FILL IN HERE *) Admitted.
+  unfold partial_function.
+  intros.
+  inversion H.
+Qed.
+
 (** [] *)
 
 (* ----------------------------------------------------------------- *)
@@ -184,7 +189,10 @@ Proof.
   unfold lt. unfold transitive.
   intros n m o Hnm Hmo.
   induction Hmo as [| m' Hm'o].
-    (* FILL IN HERE *) Admitted.
+  - apply le_S. apply Hnm.
+  - apply le_S. apply IHHm'o.
+Qed.
+
 (** [] *)
 
 (** **** Exercise: 2 stars, standard, optional (lt_trans'')
@@ -197,7 +205,12 @@ Proof.
   unfold lt. unfold transitive.
   intros n m o Hnm Hmo.
   induction o as [| o'].
-  (* FILL IN HERE *) Admitted.
+  - inversion Hmo.
+  - inversion Hmo.
+    + apply le_S. rewrite H0 in Hnm. apply Hnm.
+    + apply le_S. apply IHo'. apply H0.
+Qed.
+
 (** [] *)
 
 (** The transitivity of [le], in turn, can be used to prove some facts
@@ -215,7 +228,12 @@ Qed.
 Theorem le_S_n : forall n m,
   (S n <= S m) -> (n <= m).
 Proof.
-  (* FILL IN HERE *) Admitted.
+  intros.
+  inversion H.
+  - apply le_n.
+  - apply le_Sn_le. apply H1.
+Qed.
+
 (** [] *)
 
 (** **** Exercise: 2 stars, standard, optional (le_Sn_n_inf)
@@ -236,7 +254,13 @@ Proof.
 Theorem le_Sn_n : forall n,
   ~ (S n <= n).
 Proof.
-  (* FILL IN HERE *) Admitted.
+  unfold not.
+  intros.
+  induction n.
+  - inversion H.
+  - apply (IHn (le_S_n _ _ H)).
+Qed.
+
 (** [] *)
 
 (** Reflexivity and transitivity are the main concepts we'll need for
@@ -255,7 +279,17 @@ Definition symmetric {X: Type} (R: relation X) :=
 Theorem le_not_symmetric :
   ~ (symmetric le).
 Proof.
-  (* FILL IN HERE *) Admitted.
+  unfold not.
+  unfold symmetric.
+  intros.
+  assert (C : 1 <= 0). {
+    apply H.
+    apply le_S.
+    apply le_n.
+  }
+  apply (le_Sn_n _ C).
+Qed.
+
 (** [] *)
 
 (** A relation [R] is _antisymmetric_ if [R a b] and [R b a] together
@@ -269,7 +303,18 @@ Definition antisymmetric {X: Type} (R: relation X) :=
 Theorem le_antisymmetric :
   antisymmetric le.
 Proof.
-  (* FILL IN HERE *) Admitted.
+  unfold antisymmetric.
+  intros a b H.
+  induction H.
+  - intros. reflexivity.
+  - intros.
+    assert (C : S m <= m). {
+      apply le_trans with (b:=a).
+      apply H0. apply H.
+    }
+    destruct (le_Sn_n _ C).
+Qed.
+
 (** [] *)
 
 (** **** Exercise: 2 stars, standard, optional (le_step) *)
@@ -278,7 +323,13 @@ Theorem le_step : forall n m p,
   m <= S p ->
   n <= p.
 Proof.
-  (* FILL IN HERE *) Admitted.
+  unfold lt.
+  intros.
+  apply le_S_n.
+  apply le_trans with (b:=m).
+  apply H. apply H0.
+Qed.
+
 (** [] *)
 
 (* ----------------------------------------------------------------- *)
